We are asking you to read through a number of proofs of the same theorem.

<div class="panel panel-default">
  <div class="panel-body">
    <strong>Theorem:</strong> The sum of the first \(n\) odd integers, starting from 1, is \(n^2\).
  </div>
</div>

Expressed in algebraic notation, this theorem becomes

\[1 + 3 + 5 + 7 + \cdots + (2n-1) = \sum_{k=1}^n (2k-1) = n^2.\]

On the next page, we will show you two proofs at a time.

Please read both proofs and decide: **[JUDGING PROMPT]**

After you choose one of the proofs, you will be shown a new pair of proofs.

Please complete at least 20 of these paired comparisons.